redefine le and equiv over Pre and refactor

Rope/Basic.lean
@@ -7,15 +7,15 @@ public import Rope.WF
 -- open WF
 
 
-def Row : Type := Quotient WF.Row.instSetoid
+def Row : Type := Quotient Pre.Row.instSetoid
 
-def Ty : Type := Quotient WF.Ty.instSetoid
+def Ty : Type := Quotient Pre.Ty.instSetoid
 
-def Pred : Type := Quotient WF.Pred.instSetoid
+def Pred : Type := Quotient Pre.Pred.instSetoid
 
 -- instance : LE Row where
 --   le :=
---     Quotient.lift₂ WF.Row.le <| by
+--     Quotient.lift₂ Pre.Row.le <| by
 --       intro a1 b1 a2 b2 aeq beq
 --       cases aeq; cases beq;
 --       case _ ha1 ha2 hb1 hb2 =>
