Rope/Pre.lean
@@ -9,19 +9,19 @@ namespace Pre
 open Label
 
 -- TODO add Preds 
+-- After removing the rVar case, this now represents a ground row (but it can still contain type and label variables)
 mutual
 inductive Row : Type where
   | empty : Row -- (Identity for Concat)
-  | rVar : String -> Row
   | extend (r : Row) (l : Label)  (t : Ty) : Row
 
 inductive Ty : Type where
   | TVar (name : String) : Ty
   | TFun (arg: Ty) (ret: Ty) : Ty
   | Singleton : Label -> Ty
-  | Pi : Row -> Ty
-  | Sigma : Row -> Ty
-  | Qual : Pred -> Ty -> Ty
+  | Pi : Pre.Row -> Ty
+  | Sigma : Pre.Row -> Ty
+  | Qual : Pre.Pred -> Ty -> Ty
 
 inductive Pred : Type where
   | Contain (x: Row) (y: Row) : Pred
@@ -34,10 +34,23 @@ inductive Pred : Type where
   | TyEq (t1 t2 : Ty) : Pred
 end
 
+def Pi := Ty.Pi
+def Sigma := Ty.Sigma
+
+notation "{}" => Pre.Row.empty
+notation l " : " t " , " r => Row.extend r l t
+notation "@@" t => Ty.TVar t
+
+
+notation "''" l => Label.explicit l
+-- #check ("label" : @@"t", {})
+-- #check {} = ("hello" : (Pi {}) , {})
+
+deriving instance Repr for Row
+
 def Row.type_at (r: Row) (l: Label) : Option Ty :=
   match r with
     | .empty => .none
-    | .rVar _ => .none
     | .extend r' l' t =>
         if l = l'
         then .some t
@@ -45,7 +58,6 @@ def Row.type_at (r: Row) (l: Label) : Option Ty :=
 
 inductive Row.lack : Row -> (Label) -> Prop where
   | empty : Row.lack .empty l
-  | rVar : l ≠ l -> Row.lack (Row.rVar s) l
   | extend : Row.lack r l -> l ≠ l' -> Row.lack (extend r l' t) l
 
 theorem Row.lack_extend_lack : lack (.extend r l' t) l -> lack r l
@@ -66,8 +78,6 @@ inductive Row.disjoint : Row -> Row -> Prop where
   | refl : disjoint .empty .empty
   | extend : disjoint r1 r2 -> l1 ≠ l2 -> r1.lack l2 -> r2.lack l1 -> disjoint (.extend r1' l1 t1) (.extend r2' l2 t2)
 
-
-
 theorem Row.disjoint_symm {r1 r2 : Row} (h: Row.disjoint r1 r2) : Row.disjoint r2 r1 :=
   match h with
   | .refl => .refl
@@ -81,7 +91,6 @@ theorem Row.disjoint_symm {r1 r2 : Row} (h: Row.disjoint r1 r2) : Row.disjoint r
 
 inductive Row.unique_labels : Row -> Prop where
   | empty : unique_labels .empty
-  | rVar : unique_labels (.rVar s)
   | extend : unique_labels r -> lack r l -> unique_labels (extend r l t)
 
 theorem Row.unique_labels_lack_extend : Row.unique_labels (.extend r l t) -> Row.lack r l := by
@@ -92,8 +101,7 @@ theorem Row.unique_labels_lack_extend : Row.unique_labels (.extend r l t) -> Row
 theorem Row.unique_labels_extend {pr : Row} {l t} : Row.unique_labels (.extend pr l t) -> Row.unique_labels pr := by
   cases pr <;> intro h
   apply unique_labels.empty
-  apply unique_labels.rVar
-  cases h ;
+  cases h
   assumption
 
 -- Row is concrete (Has explicit labels and is not a variable)
@@ -101,3 +109,386 @@ theorem Row.unique_labels_extend {pr : Row} {l t} : Row.unique_labels (.extend p
 inductive Row.concrete : Row -> Prop where
   | empty : concrete .empty
   | extend : concrete r -> Label.concrete l -> lack r l -> concrete (extend r l t)
+
+inductive Row.ground : Row -> Prop where
+  | empty : ground .empty
+  | extend {r l t} : ground (extend r l t)
+  
+theorem conc_inner : Row.concrete (a.extend l t) -> Row.concrete a :=
+  by intro h; cases h; trivial
+
+-- theorem ground_inner : Row.ground (a.extend l t) -> Row.ground a :=
+--   by intro h; cases h; trivial
+
+
+theorem lacks_extend_lacks {r: Pre.Row} {l1 l2: Label} {t: Pre.Ty} (h_lack: Pre.Row.lack (r.extend l2 t) l1) : Pre.Row.lack r l1 :=
+  match h_lack with
+  | .extend h' _ => h'
+
+
+-- TODO Add Preds
+-- Well-formed rows are equivalent iff they are equal up to reordering of fields.
+-- Equivalence under a context/substitution will be defined later.
+mutual
+inductive In : Label -> Pre.Ty -> Pre.Row -> Prop where
+  | first (l: Label) (t: Pre.Ty) (a: Pre.Row) (t' : Pre.Ty) : Ty.Equiv t t' -> In l t (.extend a l t')
+  | tail (l l' : Label) (t t': Pre.Ty) (a : Pre.Row)  : In l t a -> In l t (.extend a l' t')
+  -- | equiv (l : Label) (t t' : Pre.Ty) (te : Ty.Equiv t t') (a : Pre.Row ): In l t a -> In l t' a
+
+inductive Row.le : Pre.Row -> Pre.Row -> Prop where
+  | empty {r : Pre.Row} : Row.le .empty r
+  | extendR {a b : Pre.Row} {l : Label} {t : Pre.Ty} : (a_le_b: Row.le a b) -> Row.le a (b.extend l t)
+  | extendL (a b: Pre.Row) (l : Label) (t : Pre.Ty) : (a_le_b: Row.le a b) -> (h_in : In l t b) -> Row.le (l : t, a) b
+
+-- Types are equivalent iff they are equal up to equivalence of in all subtree
+inductive Ty.Equiv : Pre.Ty  -> Pre.Ty  -> Prop where
+  | TVar : Ty.Equiv (Pre.Ty.TVar s) (Pre.Ty.TVar s)
+  | Singleton : Ty.Equiv (Pre.Ty.Singleton l) (Pre.Ty.Singleton l)
+  | Pi {a b : Pre.Row} : Row.le a b -> Row.le b a -> Ty.Equiv (.Pi a) (.Pi b)
+  | Sigma {a b : Pre.Row} : Row.le a b -> Row.le b a -> Ty.Equiv (.Sigma a) (.Sigma b)
+  | TFun : Ty.Equiv a1 a2 -> Ty.Equiv r1 r2 -> Ty.Equiv (.TFun a1 r1) (.TFun a2 r2)
+  | Qual : Pred.Equiv p1 p2 -> Ty.Equiv t1 t2 -> Ty.Equiv (.Qual p1 t1) (.Qual p2 t2)
+
+inductive Pred.Equiv : Pre.Pred -> Pre.Pred -> Prop where
+  | Contain {x1 x2 y1 y2 : Pre.Row} : Row.le x1 x2 -> Row.le x2 x1 -> Row.le y1 y2 -> Row.le y2 y1 -> Pred.Equiv (.Contain x1 y1) (.Contain x2 y2)
+    -- Garrett-style 3-place concatenation predicate
+    -- x + y ~ z
+  | Combine {x1 x2 y1 y2 z1 z2: Pre.Row} :
+    Row.le x1 x2 -> Row.le x2 x1 ->
+    Row.le y1 y2 -> Row.le y2 y1 ->
+    Row.le z1 z2 -> Row.le z2 z1 ->
+    Pred.Equiv (.Combine x1 y1 z1) (.Combine x2 y2 z2)
+  | TyEq {a1 a2 b1 b2 : Ty} : (Ty.Equiv a1 a2) -> (Ty.Equiv b1 b2) ->  Pred.Equiv (.TyEq a1 b1) (.TyEq a2 b2)
+end
+
+
+
+
+-- Probably simpler version of Row.le
+-- If we allow rVar as a case of Row, then by this definition, rVar is ≤ any row
+def Row.le' (a b : Pre.Row) := (∀ {l : Label} {t : Pre.Ty}, In l t a -> In l t b)
+
+-- def Row.le' (a b : Row) := (∀ {l : Label} {t : Pre.Ty}, In l t a.inner -> In l t b.inner)
+
+@[refl]
+theorem Row.le'.refl {a : Row} : Row.le' a a := id
+theorem Row.le'.trans {a b c : Row} : Row.le' a b -> Row.le' b c -> Row.le' a c :=
+  λ h1 h2 l t h =>
+    by
+      apply h2
+      apply h1
+      apply h
+
+instance : LE Row where
+  le := Row.le
+
+
+-- Rows are equivalent iff they are LE each other
+def Row.Equiv (a b : Row) : Prop := a ≤ b ∧ b ≤ a
+
+theorem Row.le.empty_is_refl {r : Row} : r ≤ .empty <-> r = .empty :=
+  Iff.intro (
+    λ h =>
+      match h with
+      | Row.le.empty => rfl
+  ) (
+    λ h => by
+      rw [h];
+      apply Row.le.empty)
+
+mutual
+@[refl]
+theorem Row.le.refl {x : Pre.Row} : Row.le x x :=
+  match x with
+  | .empty => .empty
+  | Pre.Row.extend r l t => by
+    apply Row.le.extendL <;> try trivial
+    apply Row.le.extendR <;> try trivial
+    apply Row.le.refl <;> trivial
+    apply In.first <;> try trivial
+    apply Ty.Equiv.refl
+
+@[refl]
+theorem Ty.Equiv.refl {t : Pre.Ty} : Ty.Equiv t t :=
+match t with
+| .TVar _ => .TVar
+| .Singleton _ => .Singleton
+| .TFun arg ret =>
+  @Ty.Equiv.TFun arg arg ret ret .refl .refl
+| .Pi _ =>
+  @Ty.Equiv.Pi _ _ .refl .refl
+| .Sigma _ =>
+  @Ty.Equiv.Sigma _ _ .refl .refl
+| .Qual _ _ => Ty.Equiv.Qual .refl .refl
+
+@[refl]
+theorem Pred.Equiv.refl {x : Pre.Pred} : Pred.Equiv x x :=
+  match x with
+  | .Contain _ _ => Pred.Equiv.Contain .refl .refl .refl .refl
+  | .Combine _ _ _ =>
+    Pred.Equiv.Combine .refl .refl .refl .refl .refl .refl
+  | .TyEq _ _ => Pred.Equiv.TyEq .refl .refl
+end
+
+@[refl]
+theorem Row.Equiv.refl {r: Row} : Row.Equiv r r :=
+  .intro .refl .refl
+
+@[symm]
+theorem Row.Equiv.symm : ∀ {x y : Row}, Row.Equiv x y → Row.Equiv y x :=
+  λ h =>
+    match h with
+    | (And.intro l r) => (And.intro r l)
+
+mutual
+@[symm]
+theorem Ty.Equiv.symm : ∀ {x y : Ty}, Ty.Equiv x y → Ty.Equiv y x :=
+  λ h =>
+    match h with
+    | .TVar => Ty.Equiv.TVar
+    | .Singleton => .Singleton
+    | .TFun h1 h2 => .TFun (Ty.Equiv.symm h1) (Ty.Equiv.symm h2)
+    | @Ty.Equiv.Pi _ _ hl hr => @.Pi _ _ hr hl
+    | @Ty.Equiv.Sigma  _ _ hl hr   => @.Sigma _ _ hr hl
+    | .Qual h1 h2 => .Qual (Pred.Equiv.symm h1) (Ty.Equiv.symm h2)
+
+@[symm]
+theorem Pred.Equiv.symm : ∀ {p q : Pred}, Pred.Equiv p q → Pred.Equiv q p :=
+  λ h =>
+    match h with
+    | .Contain a b c d => .Contain b a d c
+    | .Combine a b c d e f => .Combine b a d c f e
+    | .TyEq a b => .TyEq a.symm b.symm
+end
+
+theorem Row.le.extendL_cancel {a b : Pre.Row} (h_le : (l : t, a) ≤ b) : a ≤ b :=
+  match h_le with
+  | .extendL _ _ _ _ h _ => h
+  | .extendR _ => 
+    by
+    apply Row.le.extendR
+    apply Row.le.extendL_cancel
+    trivial
+
+
+mutual
+theorem in_equiv_in {l t1 t2} (a: Row) (h_in : In l t1 a) (e : Ty.Equiv t1 t2) : In l t2 a :=
+  match h_in with
+  | .first _ _ a' tx e' =>
+    In.first l t2 a' tx (
+    match t1, t2, tx, e, e' with
+    | .Pi a, .Pi b, .Pi c, .Pi a_le_b b_le_a, .Pi a_le_c c_le_a =>
+      Ty.Equiv.Pi (Row.le.trans b_le_a  a_le_c) (Row.le.trans c_le_a a_le_b)
+    | .Sigma _, .Sigma _, .Sigma _, .Sigma a_le_b b_le_a, .Sigma a_le_c c_le_a =>
+      Ty.Equiv.Sigma (Row.le.trans b_le_a  a_le_c) (Row.le.trans c_le_a a_le_b)
+    | .Qual p1 t1, .Qual p2 t2, .Qual p3 t3, .Qual pe te, .Qual pe' te' =>
+      Ty.Equiv.Qual (Pred.Equiv.trans pe.symm pe') (Ty.Equiv.trans te.symm te')
+    | .TFun _ _, .TFun _ _, .TFun _ _, .TFun ae re, .TFun ae' re' =>
+      Ty.Equiv.TFun (Ty.Equiv.trans ae.symm ae')  (Ty.Equiv.trans re.symm re')
+    | .Singleton _, .Singleton _, .Singleton _, .Singleton, .Singleton =>
+      .Singleton
+    | .TVar _, .TVar _, .TVar _, .TVar, .TVar => .TVar)
+  | .tail _ _ _ _ _ h_in' =>
+    by
+    apply In.tail
+    apply in_equiv_in _ h_in' e
+termination_by (sizeOf t1 + sizeOf t2 + sizeOf a)
+
+theorem in_le_in {l a b t} (h_in : In l t a) (hle : a ≤ b)   : In l t b :=
+  match h_in with
+  | .first _ _ a' t' e =>
+    have h_le_r : (l : t' , a') ≤ b := hle
+    match hle with
+    | @Row.le.extendR _ b' _ _ hle' => by
+      apply In.tail
+      apply in_le_in _ hle'
+      apply In.first _ _ _ _ e
+    | .extendL _ _ _ _ a'_le_b l_t'_in_b =>
+      in_equiv_in _ l_t'_in_b e.symm
+  | .tail _ _ _ _ a' hin' => by
+    have lem : a' ≤ b := by
+      apply Row.le.extendL_cancel hle
+    apply in_le_in hin' lem
+termination_by (sizeOf a + sizeOf b + sizeOf t)
+
+theorem Row.le.trans {a b c : Pre.Row}
+  (h_a_b : a ≤ b) (h_b_c : b ≤ c) : a ≤ c :=
+  match a, b with
+  | {}, {} => .empty
+  | {}, (lb : tb, b) => .empty
+  | (la : ta, a'), {} => (by contradiction)
+  | (la : ta, a'), (lb : tb, b') =>
+    match h_a_b with
+    | .extendL _ _ _ _ a'_le_b hin' =>
+      have hbc' : (lb : tb , b') ≤ c := h_b_c
+      match h_b_c with
+      | @Row.le.extendR  _ c' lc tc hle' =>
+        have lem'' : (la : ta, a') ≤ c' :=
+          Row.le.trans h_a_b hle'
+        have lem : a' ≤ c' :=
+          Row.le.trans a'_le_b hle'
+        have lem' : a' ≤ (lc : tc, c') :=
+          .extendR lem
+        by
+        apply Row.le.extendR lem''
+      | .extendL _ _ _ _ b'_le_c hin'' =>
+        by
+        apply Row.le.extendL _ _ _ _
+          (Row.le.trans a'_le_b hbc')
+          (in_le_in hin' hbc')
+    | .extendR a_le_b' =>
+      by
+      apply Row.le.trans a_le_b' _
+      apply Row.le.extendL_cancel h_b_c
+termination_by (sizeOf a + sizeOf b + sizeOf c)
+
+theorem Ty.Equiv.trans {x y z : Pre.Ty} :
+  Ty.Equiv x y → Ty.Equiv y z → Ty.Equiv x z :=
+  λ h1 h2 =>
+    match x, y, z with
+    | .TVar x', .TVar y', .TVar z' =>
+      by cases h1 ; cases h2; apply Ty.Equiv.refl
+    | .Singleton x', .Singleton y', .Singleton z' =>
+      by cases h1 ; cases h2; apply Ty.Equiv.refl
+    | .TFun _ _, _, _ =>
+        match h1, h2 with
+        | @Ty.Equiv.TFun _ _ _ _ h1a h1r, Ty.Equiv.TFun h2a h2r =>
+          Ty.Equiv.TFun (Ty.Equiv.trans h1a h2a) (Ty.Equiv.trans h1r h2r)
+    | .Pi a, .Pi b, .Pi c =>
+      match h1, h2 with
+      | @Ty.Equiv.Pi _ _ h_ab h_ba, Ty.Equiv.Pi h_bc h_cb => 
+        have h_ac :=
+          (@Row.le.trans a b c h_ab h_bc)
+        have h_ca :=
+          (@Row.le.trans c b a h_cb h_ba)
+        @Ty.Equiv.Pi
+        a
+        c
+        h_ac
+        h_ca
+    | .Sigma a, .Sigma b, .Sigma c =>
+      match h1, h2 with
+      | @Ty.Equiv.Sigma _ _ h_ab h_ba, Ty.Equiv.Sigma h_bc h_cb => 
+        have h_ac :=
+          (@Row.le.trans a b c h_ab h_bc)
+        have h_ca :=
+          (@Row.le.trans c b a h_cb h_ba)
+        @Ty.Equiv.Sigma
+        a
+        c
+        h_ac
+        h_ca
+    | .Qual p1 t1', .Qual p2 t2', .Qual p3 t3' =>
+      match h1, h2 with
+      | Ty.Equiv.Qual h_pxy h_txy, Ty.Equiv.Qual h_pyz h_tyz
+        =>
+          Ty.Equiv.Qual
+            (@Pred.Equiv.trans p1 p2 p3 h_pxy h_pyz)
+            (@Ty.Equiv.trans t1' t2' t3' h_txy h_tyz)
+termination_by (sizeOf x + sizeOf y + sizeOf z)
+
+theorem Pred.Equiv.trans {x y z : Pre.Pred} :
+  Pred.Equiv x y → Pred.Equiv y z → Pred.Equiv x z
+:=
+  λ h1 h2 =>
+    match y with
+    | .Contain _ _ =>
+      match h1, h2 with
+      | @Pred.Equiv.Contain _ _ _ _ ha_xy ha_yx hb_xy hb_yx,
+         Pred.Equiv.Contain ha_yz ha_zy hb_yz hb_zy =>
+          .Contain
+            (Row.le.trans ha_xy ha_yz)
+            (Row.le.trans ha_zy ha_yx)
+            (Row.le.trans hb_xy hb_yz)
+            (Row.le.trans hb_zy hb_yx)
+    | .Combine _ _ _ =>
+      match h1, h2 with
+      | @Pred.Equiv.Combine _ _ _ _ _ _ ha_xy ha_yx hb_xy hb_yx hc_xy hc_yx,
+         Pred.Equiv.Combine ha_yz ha_zy hb_yz hb_zy hc_yz hc_zy =>
+          .Combine
+            (Row.le.trans ha_xy ha_yz)
+            (Row.le.trans ha_zy ha_yx)
+            (Row.le.trans hb_xy hb_yz)
+            (Row.le.trans hb_zy hb_yx)
+            (Row.le.trans hc_xy hc_yz)
+            (Row.le.trans hc_zy hc_yx)
+    | .TyEq _ _ =>
+      match h1, h2 with
+      | @Pred.Equiv.TyEq _ _ _ _ ha_xy hb_xy,
+         Pred.Equiv.TyEq ha_yz hb_yz =>
+          .TyEq
+            (Ty.Equiv.trans ha_xy ha_yz)
+            (Ty.Equiv.trans hb_xy hb_yz)
+termination_by (sizeOf x + sizeOf y + sizeOf z)
+end
+
+
+theorem in_extend : In l t a -> In l t (l' : t', a) := by
+  intro h_in
+  apply In.tail _ _ _ _ _ h_in
+
+
+theorem Row.Equiv.trans {x y z: Row} (h_x_y : Row.Equiv x y) (h_y_z : Row.Equiv y z) : Row.Equiv x z :=
+  And.intro (Row.le.trans h_x_y.left h_y_z.left) (Row.le.trans h_y_z.right h_x_y.right)
+
+instance : Std.IsPreorder Row := ⟨λ _ => Row.le.refl, λ _ _ _ => Row.le.trans⟩
+
+
+-- This definition of equivalence is syntactic, up to reordering of fields
+-- Equivalence of rows with respect to a context or substitution will be defined over quotients of well-formed rows and types
+instance Ty.instSetoid : Setoid Ty where
+  r := Ty.Equiv
+  iseqv := ⟨λ _ => .refl, .symm, .trans⟩
+
+instance Row.instSetoid : Setoid Row where
+  r := Row.Equiv
+  iseqv := ⟨λ _ => .refl, .symm, .trans⟩
+
+instance Pred.instSetoid : Setoid Pred where
+  r := Pred.Equiv
+  iseqv := ⟨λ _ => .refl, .symm, .trans⟩
+
+
+theorem le_equiv (a b : Pre.Row) : (Row.le a b ↔ Row.le' a b) :=
+  .intro
+  (λ h l t h' =>
+    match h with
+    | Row.le.empty => by cases h'
+    | @Row.le.extendR _ b' l' t' a_le_b => by
+      rw [le_equiv] at a_le_b <;> try trivial
+      have lem : In l t b' := by
+        apply a_le_b h'
+      apply In.tail l l' t t' b' lem
+    | .extendL a' _ l' t' h_le h_in => by
+      cases h'
+      case first te =>
+        apply in_equiv_in _ h_in te.symm
+      case tail h_in' =>
+        rw [le_equiv] at h_le <;> try trivial
+        apply h_le h_in'
+  )
+  (
+    λ h =>
+      match a with
+      | .empty => .empty
+      | .extend a' la ta =>
+        match b with
+        | .empty => by
+          have lem : In la ta {} :=
+            by
+            apply h
+            apply In.first
+            apply Ty.Equiv.refl
+          cases lem
+        | .extend b' lb tb => by
+          have lem : In la ta (lb : tb , b') := by
+            apply h
+            apply In.first
+            rfl
+          have lem' : Row.le' a' (lb : tb, b') := by
+            intro lx tx hx
+            apply h
+            apply in_extend hx
+          rw [<-le_equiv] at lem'
+          apply Row.le.extendL <;> try trivial
+  )
